src/program_proof/tulip/program/gcoord/gcoord_response_session.v
@@ -1,0 +1,396 @@
+From Perennial.program_proof.tulip.program Require Import prelude.
+From Perennial.program_proof.tulip.program.gcoord Require Import
+  gcoord_repr greader_repr gpreparer_repr
+  gcoord_attached_with gcoord_receive gcoord_process_finalization_result
+  greader_process_read_result gpreparer_process_fast_prepare_result
+  gpreparer_process_validate_result gpreparer_process_prepare_result
+  gpreparer_process_unprepare_result gpreparer_process_query_result.
+
+Definition txnresp_to_val (resp : txnresp) (entsP : Slice.t) : val :=
+  match resp with
+  | ReadResp ts rid key ver =>
+      struct.mk_f TxnResponse [
+          ("Kind", #(U64 100)); ("Timestamp", #ts); ("ReplicaID", #rid);
+          ("Key", #(LitString key)); ("Version", u64_dbval_to_val ver)]
+  | FastPrepareResp ts rid res =>
+      struct.mk_f TxnResponse [
+          ("Kind", #(U64 201)); ("Timestamp", #ts); ("ReplicaID", #rid);
+          ("Result", #(rpres_to_u64 res))]
+  | ValidateResp ts rid res =>
+      struct.mk_f TxnResponse [
+          ("Kind", #(U64 202)); ("Timestamp", #ts); ("ReplicaID", #rid);
+          ("Result", #(rpres_to_u64 res))]
+  | PrepareResp ts rank rid res =>
+      struct.mk_f TxnResponse [
+          ("Kind", #(U64 203)); ("Timestamp", #ts); ("Rank", #rank);
+          ("ReplicaID", #rid); ("Result", #(rpres_to_u64 res))]
+  | UnprepareResp ts rank rid res =>
+      struct.mk_f TxnResponse [
+          ("Kind", #(U64 204)); ("Timestamp", #ts); ("Rank", #rank);
+          ("ReplicaID", #rid); ("Result", #(rpres_to_u64 res))]
+  | QueryResp ts res =>
+      struct.mk_f TxnResponse [
+          ("Kind", #(U64 205)); ("Timestamp", #ts); ("Result", #(rpres_to_u64 res))]
+  | CommitResp ts res =>
+      struct.mk_f TxnResponse [
+          ("Kind", #(U64 300)); ("Timestamp", #ts); ("Result", #(rpres_to_u64 res))]
+  | AbortResp ts res =>
+      struct.mk_f TxnResponse [
+          ("Kind", #(U64 301)); ("Timestamp", #ts); ("Result", #(rpres_to_u64 res))]
+  end.
+
+Section decode.
+  Context `{!heapGS Σ, !tulip_ghostG Σ}.
+
+  Theorem wp_DecodeTxnResponse (dataP : Slice.t) (data : list u8) (resp : txnresp) :
+    data = encode_txnresp resp ->
+    {{{ own_slice dataP byteT (DfracOwn 1) data }}}
+      DecodeTxnResponse (to_val dataP)
+    {{{ (entsP : Slice.t), RET (txnresp_to_val resp entsP);
+        (* TODO: this will be used after adding backup coordinator *)
+        match resp with
+        | _ => True
+        end
+    }}}.
+  Proof.
+    iIntros (Hdataenc Φ) "Hdata HΦ".
+    wp_rec.
+  Admitted.
+
+End decode.
+
+Section program.
+  Context `{!heapGS Σ, !tulip_ghostG Σ}.
+
+  Theorem wp_GroupCoordinator__ResponseSession
+    (gcoord : loc) (rid : u64) (addr : chan) (addrm : gmap u64 chan) gid γ :
+    addrm !! rid = Some addr ->
+    is_gcoord_with_addrm gcoord gid addrm γ -∗
+    {{{ True }}}
+      GroupCoordinator__ResponseSession #gcoord #rid
+    {{{ RET #(); True }}}.
+  Proof.
+    iIntros (Haddr) "#Hgcoord".
+    iIntros (Φ) "!> _ HΦ".
+    wp_rec.
+
+    (*@ func (gcoord *GroupCoordinator) ResponseSession(rid uint64) {           @*)
+    (*@     for {                                                               @*)
+    (*@                                                                         @*)
+    wp_apply (wp_forBreak (λ _, True)%I); wp_pures; last by iApply "HΦ".
+    clear Φ.
+    iIntros (Φ) "!> _ HΦ".
+    wp_pures.
+
+    (*@         data, ok := gcoord.Receive(rid)                                 @*)
+    (*@         if !ok {                                                        @*)
+    (*@             // Try to re-establish a connection on failure.             @*)
+    (*@             primitive.Sleep(params.NS_RECONNECT)                        @*)
+    (*@             continue                                                    @*)
+    (*@         }                                                               @*)
+    (*@                                                                         @*)
+    wp_apply (wp_GroupCoordinator__Receive with "Hgcoord").
+    { apply Haddr. }
+    iIntros (dataP ok) "Hdata".
+    wp_pures.
+    destruct ok; wp_pures; last first.
+    { wp_apply wp_Sleep.
+      wp_pures.
+      by iApply "HΦ".
+    }
+    iDestruct "Hdata" as (data resp) "(Hdata & #Hresp & %Hdataenc)".
+
+    (*@         msg := message.DecodeTxnResponse(data)                          @*)
+    (*@         kind := msg.Kind                                                @*)
+    (*@                                                                         @*)
+    wp_apply (wp_DecodeTxnResponse with "Hdata").
+    { apply Hdataenc. }
+    iIntros (entsP) "Hents".
+
+    (*@         gcoord.mu.Lock()                                                @*)
+    (*@                                                                         @*)
+    (*@         // Handle commit and abort responses. Note that timestamp check should @*)
+    (*@         // happen after.                                                @*)
+    (*@         if kind == message.MSG_TXN_COMMIT || kind == message.MSG_TXN_ABORT { @*)
+    (*@             gcoord.processFinalizationResult(msg.Timestamp, msg.Result) @*)
+    (*@             gcoord.mu.Unlock()                                          @*)
+    (*@             continue                                                    @*)
+    (*@         }                                                               @*)
+    (*@                                                                         @*)
+    (*@         // Ignore this response message if it is not the currently active one. @*)
+    (*@         if !gcoord.attachedWith(msg.Timestamp) {                        @*)
+    (*@             gcoord.mu.Unlock()                                          @*)
+    (*@             continue                                                    @*)
+    (*@         }                                                               @*)
+    (*@                                                                         @*)
+    (*@         if kind == message.MSG_TXN_READ {                               @*)
+    (*@             gcoord.grd.processReadResult(msg.ReplicaID, msg.Key, msg.Version) @*)
+    (*@         } else if kind == message.MSG_TXN_FAST_PREPARE {                @*)
+    (*@             gcoord.gpp.processFastPrepareResult(msg.ReplicaID, msg.Result) @*)
+    (*@         } else if kind == message.MSG_TXN_VALIDATE {                    @*)
+    (*@             gcoord.gpp.processValidateResult(msg.ReplicaID, msg.Result) @*)
+    (*@         } else if kind == message.MSG_TXN_PREPARE {                     @*)
+    (*@             gcoord.gpp.processPrepareResult(msg.ReplicaID, msg.Result)  @*)
+    (*@         } else if kind == message.MSG_TXN_UNPREPARE {                   @*)
+    (*@             gcoord.gpp.processUnprepareResult(msg.ReplicaID, msg.Result) @*)
+    (*@         } else if kind == message.MSG_TXN_QUERY {                       @*)
+    (*@             gcoord.gpp.processQueryResult(msg.ReplicaID, msg.Result)    @*)
+    (*@         } else if kind == message.MSG_TXN_REFRESH {                     @*)
+    (*@             // No reponse message for REFRESH.                          @*)
+    (*@         }                                                               @*)
+    (*@                                                                         @*)
+    (*@         // In the current design the coordinator will be notified whenever a new @*)
+    (*@         // response arrives, and then checks whether the final result (e.g., @*)
+    (*@         // prepared, committed, or aborted in the case of preparing) is @*)
+    (*@         // ready. An optimization would be requiring those @process{X}Result @*)
+    (*@         // functions to return a bool indicating the final result is ready, and @*)
+    (*@         // call @gcoord.cv.Signal only on those occasions.              @*)
+    (*@         gcoord.cv.Broadcast()                                           @*)
+    (*@                                                                         @*)
+    (*@         gcoord.mu.Unlock()                                              @*)
+    (*@     }                                                                   @*)
+    (*@ }                                                                       @*)
+    clear Haddr rid.
+    destruct resp; wp_pures.
+    { (* Case: TxnRead. *)
+      iNamed "Hgcoord".
+      wp_loadField.
+      wp_apply (wp_Mutex__Lock with "Hlock").
+      iIntros "[Hlocked Hgcoord]".
+      wp_pures.
+      do 2 iNamed "Hgcoord".
+      wp_apply (wp_GroupCoordinator__attachedWith with "Hgcoord").
+      iIntros (attached) "Hgcoord".
+      wp_pures.
+      destruct attached; wp_pures; last first.
+      { wp_loadField.
+        wp_apply (wp_Mutex__Unlock with "[-HΦ]").
+        { by iFrame "Hlock Hlocked ∗". }
+        wp_pures.
+        by iApply "HΦ".
+      }
+      wp_pures.
+      iNamed "Hgcoord". iNamed "Hgrd".
+      wp_loadField.
+      iNamed "Hresp".
+      wp_apply (wp_GroupReader__processReadResult with "Hsafe Hgrd").
+      { apply Hrid. }
+      iIntros "Hgrd".
+      wp_loadField.
+      wp_apply (wp_Cond__Broadcast with "Hcv").
+      wp_loadField.
+      wp_apply (wp_Mutex__Unlock with "[-HΦ]").
+      { by iFrame "Hlock Hlocked ∗". }
+      wp_pures.
+      by iApply "HΦ".
+    }
+    { (* Case: TxnFastPrepare. *)
+      iNamed "Hgcoord".
+      wp_loadField.
+      wp_apply (wp_Mutex__Lock with "Hlock").
+      iIntros "[Hlocked Hgcoord]".
+      wp_pures.
+      do 2 iNamed "Hgcoord".
+      wp_apply (wp_GroupCoordinator__attachedWith with "Hgcoord").
+      iIntros (attached) "Hgcoord".
+      wp_pures.
+      destruct attached; wp_pures; last first.
+      { wp_loadField.
+        wp_apply (wp_Mutex__Unlock with "[-HΦ]").
+        { by iFrame "Hlock Hlocked ∗". }
+        wp_pures.
+        by iApply "HΦ".
+      }
+      wp_pures.
+      iNamed "Hgcoord". iNamed "Hgpp".
+      wp_loadField.
+      iNamed "Hresp".
+      wp_apply (wp_GroupPreparer__processFastPrepareResult with "Hsafe Hinv Hgpp").
+      { apply Hgid. }
+      { apply Hrid. }
+      iIntros "Hgpp".
+      wp_loadField.
+      wp_apply (wp_Cond__Broadcast with "Hcv").
+      wp_loadField.
+      wp_apply (wp_Mutex__Unlock with "[-HΦ]").
+      { by iFrame "Hlock Hlocked ∗". }
+      wp_pures.
+      by iApply "HΦ".
+    }
+    { (* Case: TxnValdiate. *)
+      iNamed "Hgcoord".
+      wp_loadField.
+      wp_apply (wp_Mutex__Lock with "Hlock").
+      iIntros "[Hlocked Hgcoord]".
+      wp_pures.
+      do 2 iNamed "Hgcoord".
+      wp_apply (wp_GroupCoordinator__attachedWith with "Hgcoord").
+      iIntros (attached) "Hgcoord".
+      wp_pures.
+      destruct attached; wp_pures; last first.
+      { wp_loadField.
+        wp_apply (wp_Mutex__Unlock with "[-HΦ]").
+        { by iFrame "Hlock Hlocked ∗". }
+        wp_pures.
+        by iApply "HΦ".
+      }
+      wp_pures.
+      iNamed "Hgcoord". iNamed "Hgpp".
+      wp_loadField.
+      iNamed "Hresp".
+      wp_apply (wp_GroupPreparer__processValidateResult with "Hsafe Hinv Hgpp").
+      { apply Hgid. }
+      { apply Hrid. }
+      iIntros "Hgpp".
+      wp_loadField.
+      wp_apply (wp_Cond__Broadcast with "Hcv").
+      wp_loadField.
+      wp_apply (wp_Mutex__Unlock with "[-HΦ]").
+      { by iFrame "Hlock Hlocked ∗". }
+      wp_pures.
+      by iApply "HΦ".
+    }
+    { (* Case: TxnPrepare. *)
+      iNamed "Hgcoord".
+      wp_loadField.
+      wp_apply (wp_Mutex__Lock with "Hlock").
+      iIntros "[Hlocked Hgcoord]".
+      wp_pures.
+      do 2 iNamed "Hgcoord".
+      wp_apply (wp_GroupCoordinator__attachedWith with "Hgcoord").
+      iIntros (attached) "Hgcoord".
+      wp_pures.
+      destruct attached; wp_pures; last first.
+      { wp_loadField.
+        wp_apply (wp_Mutex__Unlock with "[-HΦ]").
+        { by iFrame "Hlock Hlocked ∗". }
+        wp_pures.
+        by iApply "HΦ".
+      }
+      case_bool_decide as Hrank; wp_pures.
+      { inv Hrank.
+        iNamed "Hgcoord". iNamed "Hgpp".
+        wp_loadField.
+        iNamed "Hresp".
+        wp_apply (wp_GroupPreparer__processPrepareResult with "Hsafe Hgpp").
+        { apply Hrid. }
+        iIntros "Hgpp".
+        wp_loadField.
+        wp_apply (wp_Cond__Broadcast with "Hcv").
+        wp_loadField.
+        wp_apply (wp_Mutex__Unlock with "[-HΦ]").
+        { by iFrame "Hlock Hlocked ∗". }
+        wp_pures.
+        by iApply "HΦ".
+      }
+      wp_loadField.
+      wp_apply (wp_Cond__Broadcast with "Hcv").
+      wp_loadField.
+      wp_apply (wp_Mutex__Unlock with "[-HΦ]").
+      { by iFrame "Hlock Hlocked ∗". }
+      wp_pures.
+      by iApply "HΦ".
+    }
+    { (* Case: TxnUnprepare. *)
+      iNamed "Hgcoord".
+      wp_loadField.
+      wp_apply (wp_Mutex__Lock with "Hlock").
+      iIntros "[Hlocked Hgcoord]".
+      wp_pures.
+      do 2 iNamed "Hgcoord".
+      wp_apply (wp_GroupCoordinator__attachedWith with "Hgcoord").
+      iIntros (attached) "Hgcoord".
+      wp_pures.
+      destruct attached; wp_pures; last first.
+      { wp_loadField.
+        wp_apply (wp_Mutex__Unlock with "[-HΦ]").
+        { by iFrame "Hlock Hlocked ∗". }
+        wp_pures.
+        by iApply "HΦ".
+      }
+      case_bool_decide as Hrank; wp_pures.
+      { inv Hrank.
+        iNamed "Hgcoord". iNamed "Hgpp".
+        wp_loadField.
+        iNamed "Hresp".
+        wp_apply (wp_GroupPreparer__processUnprepareResult with "Hsafe Hgpp").
+        { apply Hrid. }
+        iIntros "Hgpp".
+        wp_loadField.
+        wp_apply (wp_Cond__Broadcast with "Hcv").
+        wp_loadField.
+        wp_apply (wp_Mutex__Unlock with "[-HΦ]").
+        { by iFrame "Hlock Hlocked ∗". }
+        wp_pures.
+        by iApply "HΦ".
+      }
+      wp_loadField.
+      wp_apply (wp_Cond__Broadcast with "Hcv").
+      wp_loadField.
+      wp_apply (wp_Mutex__Unlock with "[-HΦ]").
+      { by iFrame "Hlock Hlocked ∗". }
+      wp_pures.
+      by iApply "HΦ".
+    }
+    { (* Case: TxnQuery. *)
+      iNamed "Hgcoord".
+      wp_loadField.
+      wp_apply (wp_Mutex__Lock with "Hlock").
+      iIntros "[Hlocked Hgcoord]".
+      wp_pures.
+      do 2 iNamed "Hgcoord".
+      wp_apply (wp_GroupCoordinator__attachedWith with "Hgcoord").
+      iIntros (attached) "Hgcoord".
+      wp_pures.
+      destruct attached; wp_pures; last first.
+      { wp_loadField.
+        wp_apply (wp_Mutex__Unlock with "[-HΦ]").
+        { by iFrame "Hlock Hlocked ∗". }
+        wp_pures.
+        by iApply "HΦ".
+      }
+      wp_pures.
+      iNamed "Hgcoord". iNamed "Hgpp".
+      wp_loadField.
+      iNamed "Hresp".
+      wp_apply (wp_GroupPreparer__processQueryResult with "Hresp Hgpp").
+      iIntros "Hgpp".
+      wp_loadField.
+      wp_apply (wp_Cond__Broadcast with "Hcv").
+      wp_loadField.
+      wp_apply (wp_Mutex__Unlock with "[-HΦ]").
+      { by iFrame "Hlock Hlocked ∗". }
+      wp_pures.
+      by iApply "HΦ".
+    }
+    { iNamed "Hgcoord".
+      wp_loadField.
+      wp_apply (wp_Mutex__Lock with "Hlock").
+      iIntros "[Hlocked Hgcoord]".
+      wp_pures.
+      do 3 iNamed "Hgcoord".
+      wp_apply (wp_GroupCoordinator__processFinalizationResult with "Hgfl").
+      iIntros "Hgfl".
+      wp_loadField.
+      wp_apply (wp_Mutex__Unlock with "[-HΦ]").
+      { by iFrame "Hlock Hlocked ∗". }
+      wp_pures.
+      by iApply "HΦ".
+    }
+    { iNamed "Hgcoord".
+      wp_loadField.
+      wp_apply (wp_Mutex__Lock with "Hlock").
+      iIntros "[Hlocked Hgcoord]".
+      wp_pures.
+      do 3 iNamed "Hgcoord".
+      wp_apply (wp_GroupCoordinator__processFinalizationResult with "Hgfl").
+      iIntros "Hgfl".
+      wp_loadField.
+      wp_apply (wp_Mutex__Unlock with "[-HΦ]").
+      { by iFrame "Hlock Hlocked ∗". }
+      wp_pures.
+      by iApply "HΦ".
+    }
+  Qed.
+
+End program.
