src/program_proof/tulip/program/gcoord/gcoord_send.v
@@ -1,21 +1,166 @@
 From Perennial.program_proof.tulip.program Require Import prelude.
-From Perennial.program_proof.tulip.program.gcoord Require Import gcoord_repr.
+From Perennial.program_proof.tulip.program.gcoord Require Import
+  gcoord_repr gcoord_get_connection gcoord_connect.
+
+Section encode.
+  Context `{!heapGS Σ, !paxos_ghostG Σ}.
+
+  Theorem wp_EncodeTxnReadRequest (ts : u64) (key : string) :
+    {{{ True }}}
+      EncodeTxnReadRequest #ts #(LitString key)
+    {{{ (dataP : Slice.t) (data : list u8), RET (to_val dataP);
+        own_slice dataP byteT (DfracOwn 1) data ∗
+        ⌜data = encode_txnreq (ReadReq ts key)⌝
+    }}}.
+  Proof.
+  Admitted.
+
+End encode.
 
 Section program.
   Context `{!heapGS Σ, !tulip_ghostG Σ}.
 
+  Theorem wp_GroupCoordinator__Send
+    (gcoord : loc) (rid : u64) (dataP : Slice.t) (data : list u8)
+    (addrm : gmap u64 chan) (addr : chan) gid γ :
+    addrm !! rid = Some addr ->
+    is_gcoord_with_addrm gcoord gid addrm γ -∗
+    {{{ own_slice dataP byteT (DfracOwn 1) data }}}
+    <<< ∀∀ ms, addr c↦ ms >>>
+      GroupCoordinator__Send #gcoord #rid (to_val dataP) @ ∅
+    <<< ∃∃ (ok : bool),
+            if ok
+            then ∃ trml, addr c↦ ({[Message trml data]} ∪ ms) ∗ is_terminal γ gid trml
+            else addr c↦ ms
+    >>>
+    {{{ RET #(); True }}}.
+  Proof.
+    iIntros (Haddr) "#Hgcoord".
+    iIntros (Φ) "!> Hdata HAU".
+    wp_rec.
+
+    (*@ func (gcoord *GroupCoordinator) Send(rid uint64, data []byte) {         @*)
+    (*@     conn, ok := gcoord.GetConnection(rid)                               @*)
+    (*@     if !ok {                                                            @*)
+    (*@         gcoord.Connect(rid)                                             @*)
+    (*@         return                                                          @*)
+    (*@     }                                                                   @*)
+    (*@                                                                         @*)
+    wp_apply (wp_GroupCoordinator__GetConnection with "Hgcoord").
+    { apply Haddr. }
+    iIntros (trml ok) "#Htrmlrcpt".
+    wp_pures.
+    destruct ok; wp_pures; last first.
+    { wp_apply (wp_GroupCoordinator__Connect with "Hgcoord").
+      { apply Haddr. }
+      iIntros (ok) "Hok".
+      wp_pures.
+      (* Open the AU without updating. *)
+      iMod (ncfupd_mask_subseteq (⊤ ∖ ∅)) as "Hclose"; first solve_ndisj.
+      iMod "HAU" as (ms) "[Hms HAU]".
+      iMod ("HAU" $! false with "Hms") as "HΦ".
+      iMod "Hclose" as "_".
+      by iApply "HΦ".
+    }
+
+    (*@     err := grove_ffi.Send(conn, data)                                   @*)
+    (*@     if err {                                                            @*)
+    (*@         gcoord.Connect(rid)                                             @*)
+    (*@     }                                                                   @*)
+    (*@ }                                                                       @*)
+    iDestruct (own_slice_to_small with "Hdata") as "Hdata".
+    wp_apply (wp_Send with "Hdata").
+    iMod "HAU" as (ms) "[Hms HAU]".
+    iFrame "Hms".
+    iIntros "!>" (sent) "Hms".
+    iMod ("HAU" $! sent with "[Hms]") as "HΦ".
+    { rewrite union_comm_L. by destruct sent; first iFrame. }
+    iModIntro.
+    iIntros (err) "[%Herr Hdata]".
+    wp_pures.
+    wp_if_destruct.
+    { wp_apply (wp_GroupCoordinator__Connect with "Hgcoord").
+      { apply Haddr. }
+      iIntros (ok) "_".
+      wp_pures.
+      by iApply "HΦ".
+    }
+    by iApply "HΦ".
+  Qed.
 
   Theorem wp_GroupCoordinator__SendRead
-    (gcoord : loc) (rid : u64) (ts : u64) (key : string) gid γ :
-    is_gcoord gcoord gid γ -∗
+    (gcoord : loc) (rid : u64) (ts : u64) (key : string) addrm gid γ :
+    safe_read_req gid (uint.nat ts) key ->
+    rid ∈ dom addrm ->
+    is_gcoord_with_addrm gcoord gid addrm γ -∗
     {{{ True }}}
       GroupCoordinator__SendRead #gcoord #rid #ts #(LitString key)
     {{{ RET #(); True }}}.
   Proof.
+    iIntros (Hrid Hsafe) "#Hgcoord".
+    iIntros (Φ) "!> _ HΦ".
+    wp_rec.
+
     (*@ func (gcoord *GroupCoordinator) SendRead(rid, ts uint64, key string) {  @*)
     (*@     gcoord.Send(rid, message.EncodeTxnRead(ts, key))                    @*)
     (*@ }                                                                       @*)
-  Admitted.
+    wp_apply (wp_EncodeTxnReadRequest).
+    iIntros (dataP data) "[Hdata %Hdataenc]".
+    iNamed "Hgcoord".
+    iNamed "Haddrm".
+    assert (is_Some (addrm !! rid)) as [addrpeer Haddrpeer].
+    { by apply elem_of_dom. }
+    wp_apply (wp_GroupCoordinator__Send with "[] Hdata"); first apply Haddrpeer.
+    { iFrame "# %". }
+    iInv "Hinvnet" as "> HinvnetO" "HinvnetC".
+    iApply ncfupd_mask_intro; first set_solver.
+    iIntros "Hmask".
+    iNamed "HinvnetO".
+    assert (is_Some (listens !! addrpeer)) as [ms Hms].
+    { rewrite -elem_of_dom -Himgaddrm elem_of_map_img. by eauto. }
+    iDestruct (big_sepM_delete with "Hlistens") as "[Hlst Hlistens]"; first apply Hms.
+    iNamed "Hlst".
+    iFrame "Hms".
+    iIntros (sent) "Hms".
+    destruct sent; last first.
+    { iDestruct (big_sepM_insert_2 _ _ addrpeer ms with "[Hms] Hlistens") as "Hlistens".
+      { iFrame "∗ # %". }
+      rewrite insert_delete; last apply Hms.
+      iMod "Hmask" as "_".
+      iMod ("HinvnetC" with "[$Hlistens $Hconnects $Hterminals]") as "_".
+      { done. }
+      iIntros "!> _".
+      wp_pures.
+      by iApply "HΦ".
+    }
+    iDestruct "Hms" as (trml) "[Hms #Htrml]".
+    set ms' := _ ∪ ms.
+    iDestruct (big_sepM_insert_2 _ _ addrpeer ms' with "[Hms] Hlistens") as "Hlistens".
+    { iFrame "Hms".
+      set req := ReadReq _ _ in Hdataenc.
+      iExists ({[req]} ∪ reqs).
+      iSplit.
+      { rewrite set_map_union_L set_map_singleton_L.
+        by iApply big_sepS_insert_2.
+      }
+      iSplit.
+      { iApply big_sepS_insert_2; [done | done]. }
+      iPureIntro.
+      rewrite 2!set_map_union_L 2!set_map_singleton_L /= -Hdataenc.
+      set_solver.
+    }
+    rewrite insert_delete_insert.
+    iMod "Hmask" as "_".
+    iMod ("HinvnetC" with "[$Hlistens $Hconnects $Hterminals]") as "_".
+    { iPureIntro.
+      rewrite dom_insert_L Himgaddrm.
+      apply (elem_of_map_img_2 (SA := gset chan)) in Haddrpeer.
+      set_solver.
+    }
+    iIntros "!> _".
+    wp_pures.
+    by iApply "HΦ".
+  Qed.
 
   Theorem wp_GroupCoordinator__SendFastPrepare
     (gcoord : loc) (rid : u64) (ts : u64) (pwrsP : loc) (ptgsP : Slice.t) gid γ :
