src/program_proof/tulip/program/replica/replica_refresh.v
@@ -1,0 +1,21 @@
+From Perennial.program_proof.tulip.program Require Import prelude.
+From Perennial.program_proof.tulip.program.replica Require Import
+  replica_repr replica_finalized replica_last_proposal replica_acquire
+  replica_accept replica_log.
+
+Section program.
+  Context `{!heapGS Σ, !tulip_ghostG Σ}.
+
+  Theorem wp_Replica__refresh (rp : loc) (ts : u64) (rank : u64) gid rid γ α :
+    {{{ own_replica rp gid rid γ α }}}
+      Replica__refresh #rp #ts #rank
+    {{{ RET #(); own_replica rp gid rid γ α }}}.
+  Proof.
+    iIntros (Φ) "Hrp HΦ".
+    wp_rec. wp_pures. by iApply "HΦ".
+    (*@ func (rp *Replica) refresh(ts uint64, rank uint64) {                    @*)
+    (*@     // TODO                                                             @*)
+    (*@ }                                                                       @*)
+  Qed.
+
+End program.
